Added the two missing examples of the paper

src/Examples.v
@@ -76,3 +76,149 @@ Proof with (unfold A, B, Entry; simpl; eauto with typ).
     + eapply t_new_hot...
     + eapply t_new_hot...
 Qed.
+
+
+(* ------------------------------------------------------------------------ *)
+(** ** Example 2 *)
+(*
+
+class ConstStream () {
+ var tail = this
+}
+
+class Entry () {
+ def main() {
+   new ConstStream()
+ }
+}
+
+*)
+
+(** ** Definitions *)
+(* To put in Language.v *)
+
+
+Definition ConstStream := cln(1).
+Definition Entry := cln(0).
+Definition EntryClass :=
+  class nil nil (fun m => if (let 'mtd n := m in PeanoNat.Nat.eqb n 0)
+                       then Some (method hot nil (ConstStream,hot) (e_new ConstStream nil))
+                       else None).
+
+Definition Ξ : list Class :=
+  [(* Main Class *)
+    EntryClass;
+
+    (* Class ConstStream *)
+    class nil [field (ConstStream, cold) (e_this)] (fun _ => None)
+  ].
+
+Lemma EntryClass_ct : ct Entry = EntryClass.
+Proof. unfold ct, Entry. simpl. reflexivity. Qed.
+
+(** ** Typing *)
+(* To put in Soundness.v *)
+
+Lemma typable_classes : T_Classes.
+Proof with (unfold ConstStream, Entry; simpl; eauto with typ).
+  unfold T_Classes.
+  intros [c].
+  assert (c = 1 \/ (c = 0 \/ c > 1)) as [|] by lia; subst; simpl.
+  - (* Class ConstStream *)
+    split.
+    + eapply t_fields_cool_cons; eauto using T_Fields.
+      simpl...
+    + intros. inverts H.
+  - (* Class Entry *)
+    assert (P_hots []) by (unfold P_hots; eauto using Forall).
+    steps; try lia...
+    all: try eapply t_new_hot...
+Qed.
+
+
+(* ------------------------------------------------------------------------ *)
+(** ** Example 3 *)
+(*
+
+class Server (a : Address) {
+ var address : (Address: hot) = a
+ var _ = this.broadcast()
+
+ @ cool{address} def broadcast() : (Address: hot) = { this.address }
+}
+
+class Address () { }
+
+class Entry () {
+ def main() {
+   new Server(new Address())
+ }
+}
+
+*)
+
+(** ** Definitions *)
+(* To put in Language.v *)
+
+
+Definition Server := cln(1).
+Definition Address := cln(2).
+Definition Entry := cln(0).
+
+Definition EntryClass :=
+  class nil nil (fun m => if (let 'mtd n := m in PeanoNat.Nat.eqb n 0)
+                       then Some (method hot nil (Server,hot) (e_new Server [e_new Address []]))
+                       else None).
+
+Definition Ξ : list Class :=
+  [(* Main Class *)
+    EntryClass;
+
+    (* Class Server *)
+    class [(Address, hot)] [field (Address, hot) (e_var 0); field (Address, hot) (e_mtd (e_this) (mtd 0) nil)]
+      (fun m => if (let 'mtd n := m in PeanoNat.Nat.eqb n 0)
+                       then Some (method (cool 1) nil (Address,hot) (e_fld e_this 0))
+                       else None);
+
+    (* Class Adress *)
+    class nil nil (fun _ => None)
+  ].
+
+Lemma EntryClass_ct : ct Entry = EntryClass.
+Proof. unfold ct, Entry. simpl. reflexivity. Qed.
+Definition main: Mtd := mtd(0).
+
+(** ** Typing *)
+(* To put in Soundness.v *)
+
+
+Lemma typable_classes : T_Classes.
+Proof with (unfold Address, Server, Entry; simpl; eauto with typ lia).
+  unfold T_Classes. intros C.
+  assert (C = Address \/ C = Server \/ ct C = ct Entry). {
+    destruct C as [c].
+    assert (c = 1 \/ c = 2 \/ (c = 0 \/ c > 2)) as [|[|[|]]] by lia;
+      subst; unfold Address, Server, Entry; simpl; auto.
+    right. right. repeat (destruct c; try lia; auto).
+  }
+  destruct H as [|[|]]; rewrite H; subst...
+  - (* Class Address *)
+    split.
+    + eapply t_fields_nil.
+    + intros. inverts H.
+  - (* Class Server *)
+    split.
+    + eapply t_fields_cool_cons; eauto using T_Fields; simpl...
+      eapply t_fields_cool_cons; eauto using T_Fields; simpl.
+      eapply t_call with (C := cln 1) (μ0 := cool 1); steps...
+    + intros.
+      destruct m. steps...
+  - (* Class Entry *)
+    assert (P_hots []) by (unfold P_hots; eauto using Forall).
+    unfold Entry in *.
+    split; [eauto using T_Fields | steps].
+    unfold Server, Address.
+    eapply t_new_hot with (argsTs:=[(cln 2, hot)]); steps...
+    eapply t_exprs_cons...
+    eapply t_new_hot...
+Qed.
